src/Narcissus/Examples/NetworkStack/UDP_Packet.v
@@ -35,7 +35,7 @@ Section UDP_Decoder.
   (* These values are provided by the IP header for checksum calculation.*)
   Variable srcAddr : Vector.t (word 8) 4.
   Variable destAddr : Vector.t (word 8) 4.
-  Variable udpLength : Vector.t (word 8) 2.
+  Variable udpLength : word 16.
 
   Record UDP_Packet :=
     { SourcePort : word 16;
